links

theories/PostsTheorem/TuringJump.v
@@ -101,28 +101,30 @@ Section halting.
 
 End halting.
 
-Module Ξ.
+Section Enumerator.
   (** ** Enumerating Oracle Machines *)
 
   Context {Part : partiality}.
 
-  Variable EPF_assm : EPF.
+  Axiom EPF_assm : EPF.
   Definition θ := proj1_sig EPF_assm.
   Definition EPF := proj2_sig EPF_assm.
 
-  Variable iota1 : (nat * list bool) -> nat.
-  Variable iota2 : (nat + unit) -> nat.
-  Variable rho1 : nat -> nat * list bool.
-  Variable rho2 : nat -> nat + unit.
+  Variable O : Type.
 
-  Variable bij1 : forall y, (rho1 (iota1 y) = y).
-  Variable bij2 : forall y, (rho2 (iota2 y) = y).
+  Parameter iota1 : (nat * list bool) -> nat.
+  Parameter iota2 : (nat + O) -> nat.
+  Parameter rho1 : nat -> nat * list bool.
+  Parameter rho2 : nat -> nat + O.
 
-  Definition ξ : nat -> nat -> tree nat bool unit :=
+  Parameter bij1 : forall y, (rho1 (iota1 y) = y).
+  Parameter bij2 : forall y, (rho2 (iota2 y) = y).
+
+  Definition ξ : nat -> nat -> tree nat bool O :=
     fun c x l => bind (θ c (iota1 (x, l))) (fun v => ret (rho2 v)).
 
   Lemma ξ_parametric :
-    forall τ : nat -> nat -> tree nat bool unit, exists γ, forall n l i o, ξ (γ n) i l =! o <-> τ n i l =! o.
+    forall τ : nat -> nat -> tree nat bool O, exists γ, forall n l i o, ξ (γ n) i l =! o <-> τ n i l =! o.
   Proof.
     intros τ.
     destruct (EPF (fun n x => let (i,l) := rho1 x in bind (τ n i l) (fun v => ret (iota2 v)))) as [γ H].
@@ -137,22 +139,28 @@ Module Ξ.
     repeat eexists. eauto. eapply bij2.
   Qed.
 
-  Fact ξ_surjective (τ : nat -> tree nat bool unit) :
+  Fact ξ_surjective (τ : nat -> tree nat bool O) :
     exists j, forall l i o, ξ j i l =! o <-> τ i l =! o.
   Proof.
     destruct (ξ_parametric (fun _ => τ)) as [γ Hγ].
     now exists (γ 42).
   Qed.
 
+End Enumerator.
+
+Section SemiDecEnumerator.
+
+  Context {Part : partiality}.
+
   Definition rel {I A Q} (τ : I -> list A ↛ (Q + unit)) R x :=
     exists qs ans, interrogation (τ x) R qs ans /\ (τ x) ans =! inr tt.
 
-  Definition Ξ c R x := rel (ξ c) R x.
+  Definition Ξ c R x := rel (ξ unit c) R x.
 
   Fact computable :
     OracleComputable (fun R '(c,x) (o : unit) => Ξ c R x).
   Proof.
-    exists (fun '(c,x) => ξ c x). intros R [c x] [].
+    exists (fun '(c,x) => ξ unit c x). intros R [c x] [].
     reflexivity.
   Qed.
 
@@ -180,15 +188,48 @@ Module Ξ.
     - exists (γ 27). intros. rewrite Hτ Hγ. reflexivity.
   Qed.
 
-End Ξ.
+End SemiDecEnumerator.
+
+Section TuringRedEnumerator.
+
+  Context {Part : partiality}.
+
+  Definition rel_b {I A Q} (τ : I -> list A ↛ (Q + bool)) R x o :=
+    exists qs ans, interrogation (τ x) R qs ans /\ (τ x) ans =! inr o.
+
+  Definition χ c R x := rel_b (ξ bool c) R x.
+
+  Fact computable_b :
+    OracleComputable (fun R '(c,x) (o : unit) => Ξ c R x).
+  Proof.
+    exists (fun '(c,x) => ξ unit c x). intros R [c x] [].
+    reflexivity.
+  Qed.
+
+  Fact surjective_b (F : (nat -> bool -> Prop) -> nat -> bool -> Prop) (H : OracleComputable F) :
+    exists c, forall R x b, χ c R x b <-> F R x b.
+  Proof.
+    destruct H as [τ Hτ].
+    destruct (ξ_surjective τ) as [c Hc].
+    exists c. intros. unfold χ, rel_b.
+    setoid_rewrite Hτ. setoid_rewrite Hc.
+    firstorder.
+    exists x0, x1. split; eauto. eapply interrogation_ext. 2: reflexivity. 2: eassumption.
+    firstorder.
+    exists x0, x1. split; eauto. eapply interrogation_ext. 2: reflexivity. 2: eauto.
+    firstorder.
+  Qed.
+
+End TuringRedEnumerator.
 
 (* Opaque Ξ.Ξ. *)
-Notation Ξ := Ξ.Ξ.
 
 Notation oracle_semi_decidable := OracleSemiDecidable.
 
 Section jump.
   (** ** Synthetic Turing Jump *)
+
+  Context {Part : partiality}.
 
   Definition J Q c := Ξ c (char_rel Q) c.
 
@@ -197,7 +238,7 @@ Section jump.
     exists (fun O c o => Ξ c O c). split.
     - eapply OracleComputable_ext.
       eapply computable_bind.
-      2: eapply Ξ.computable. 2: cbn.
+      2: eapply computable. 2: cbn.
       eapply computable_ident. cbn.
       intros ? ? []; firstorder subst.
       firstorder.
@@ -207,7 +248,7 @@ Section jump.
   Lemma not_semidecidable_compl_J Q : ~ oracle_semi_decidable Q (compl (J Q)).
   Proof.
     intros (F & Hcomp & H). 
-    specialize (Ξ.surjective Hcomp) as [c Hc].
+    specialize (surjective Hcomp) as [c Hc].
     unfold J in H. specialize (H c).
     rewrite <- Hc in H. tauto.
   Qed.
@@ -221,7 +262,7 @@ Section jump.
   Proof.
     split.
     - assert (OracleComputable (fun R (x : nat) (o : unit) => R x true))
-               as [c Hc] % Ξ.surjective.
+               as [c Hc] % surjective.
       { eapply OracleComputable_ext.
         eapply computable_bind. eapply computable_id.
         eapply computable_if with (test := snd).
@@ -247,7 +288,7 @@ Section jump.
   Lemma red_𝒥_J_self Q : 
     𝒥 Q ⪯ₘ J Q.
   Proof.
-    destruct (Ξ.parametric (fun! ⟨c,x⟩ => fun _ => Ξ.ξ c x)) as [γ Hγ].
+    destruct (parametric (fun! ⟨c,x⟩ => fun _ => ξ unit c x)) as [γ Hγ].
     exists γ. unfold J, 𝒥. red. setoid_rewrite Hγ. intros ⟨c, x⟩.
     reflexivity. 
   Qed.
@@ -257,7 +298,7 @@ Section jump.
   Proof.
     split.
     - intros [F [Hom H]]. apply red_m_transitive with (𝒥 Q). 2: apply red_𝒥_J_self.
-      specialize (Ξ.surjective Hom) as [c Hc].
+      specialize (surjective Hom) as [c Hc].
       unfold 𝒥.
       exists (fun x => embed (c, x)).
       intros x. rewrite H. rewrite embedP. now rewrite Hc.
@@ -269,7 +310,7 @@ Section jump.
       + eapply OracleComputable_ext.
         eapply computable_bind.
         2: eapply computable_precompose with (g := fun '(c, i) => (f c, f i)).
-        2: eapply Ξ.computable.
+        2: eapply computable.
         2: cbn.
         eapply computable_ident.
         intros ? ? []. firstorder subst. firstorder.
@@ -321,7 +362,7 @@ End jump.
 Notation "A '´'" := (J A) (at level 20, format "A ´").
 Notation "­{0}" := (fun x:nat => x=0).
 
-Fixpoint jump_n Q n :=
+Fixpoint jump_n {Part : partiality} Q n :=
   match n with
   | 0 => Q
   | S n => J (jump_n Q n)
